4.5: Read method

Lab3_circular_buffer_template.dfy
@@ -13,6 +13,7 @@ class CircularMemory
     ensures read_position == 0
     ensures write_position == 0
     ensures !isFlipped
+    ensures Valid()
   {
     cells := new int[cap];
     read_position, write_position := 0, 0;
@@ -28,23 +29,38 @@ class CircularMemory
        (!isFlipped ==> read_position <= write_position)
   }
 
+  predicate isEmpty()
+     reads this
+  {
+       !isFlipped && write_position == read_position
+  }
+
+  predicate isFull()
+     reads this
+  {
+       isFlipped
+  }
+
 
   method Read() returns (isSuccess : bool, content : int)
     modifies this
     requires Valid()
     ensures  Valid()
-    ensures  isSuccess ==> ...
-    ensures !isSuccess ==> ...
+    ensures  isSuccess ==> old(read_position) + 1 = read_position
+    ensures !isSuccess ==> old(read_position) = read_position
 
-  {
-    if(isFlipped)
+   
+    var isSuccess: bool = false;
+    var content: int = 0;
+     
+    if(!isFlipped && write_position == read_position)
     {
-      ...
+         return;
     }
-    else // not flipped
-    {
-      ...
-    }
+
+    content := cells[read_position];       
+    read_position := read_position + 1;
+    isSuccess := true;
   }
 
   method Write(input : int) returns (isSuccess : bool)
